Liveness insensitivity (requested by @nikswamy)

ulib/FStar.ModifiesGen.fst
@@ -540,6 +540,28 @@ let loc_disjoint_regions #al #c rs1 rs2 =
   assert (loc_aux_disjoint (Ghost.reveal (Loc?.aux (loc_regions #_ #c rs1))) (Ghost.reveal (Loc?.aux (loc_regions #_ #c rs2))))
 
 
+(** Liveness-insensitive memory locations *)
+
+let liveness_insensitive_region_liveness_tags (#aloc: aloc_t) (#c: cls aloc) (l: loc c) : GTot Type0 =
+  Set.subset (Ghost.reveal (Loc?.region_liveness_tags l)) Set.empty
+
+let liveness_insensitive_region_addresses (#aloc: aloc_t) (#c: cls aloc) (l: loc c) : GTot Type0 =
+  (forall (r: HS.rid { Set.mem r (regions_of_loc l) }) . Set.subset (Loc?.non_live_addrs l r) Set.empty)
+
+let liveness_insensitive' (#aloc: aloc_t) (#c: cls aloc) (l: loc c) : GTot Type0 =
+  liveness_insensitive_region_addresses l /\
+  liveness_insensitive_region_liveness_tags l
+
+let liveness_insensitive = liveness_insensitive'
+
+let liveness_insensitive_aloc #al #c #r #n a = ()
+
+let liveness_insensitive_addresses #al c r a = ()
+
+let liveness_insensitive_union #al #c l1 l2 =
+  assert (forall (r: HS.rid { Set.mem r (regions_of_loc l1) } ) . Set.subset (Loc?.non_live_addrs l1 r) (Loc?.non_live_addrs (loc_union l1 l2) r));
+  assert (forall (r: HS.rid { Set.mem r (regions_of_loc l2) } ) . Set.subset (Loc?.non_live_addrs l2 r) (Loc?.non_live_addrs (loc_union l1 l2) r))
+
 (** The modifies clause proper *)
 
 let modifies_preserves_livenesses
@@ -736,6 +758,8 @@ let modifies_loc_includes #al #c s1 h h' s2 =
   Classical.forall_intro_2 (loc_aux_disjoint_sym #al #c);
   Classical.forall_intro_3 (fun l1 l2 l3 -> Classical.move_requires (loc_aux_disjoint_loc_aux_includes #al #c l1 l2) l3);
   assert (modifies_preserves_alocs s1 h h')
+
+let modifies_preserves_liveness #al #c s1 s2 h h' #t #pre r = ()
 
 let modifies_trans'
   (#al: aloc_t) (#c: cls al)
